everything compiles, and PipelineTest can display the instructions that the compiler outputs when compiling fib6

src/NameGen.v
@@ -49,3 +49,26 @@ Instance NatNameGen: NameGen nat (nat -> Prop) nat := {|
 Defined.
 (* We use "abstract" to make the proofs opaque, but "Defined" to make sure that
    "genFresh" and "allFreshVars" are transparent for reduction. *)
+
+
+Definition listmaxZ(l: list Z): Z := fold_right Z.max 0%Z l.
+
+Lemma listmaxZ_spec: forall l v, In v l -> (v <= listmaxZ l)%Z.
+Proof.
+  induction l; intros.
+  - simpl in H. contradiction.
+  - simpl in *. destruct H.
+    + subst. apply Z.le_max_l. 
+    + pose proof (Z.le_max_r a (listmaxZ l)).
+      specialize (IHl v H).
+      eapply Z.le_trans; eassumption.
+Qed.
+
+Instance ZNameGen: NameGen Z (Z -> Prop) Z := {|
+  freshNameGenState := fun l => (listmaxZ l + 1)%Z;
+  genFresh := fun s => (s, (s + 1)%Z);
+  allFreshVars := fun s => fun x => (s <= x)%Z
+|}.
+  abstract (intros; inversion H; subst; unfold subset; simpl; intuition omega).
+  abstract (unfold contains, Function_Set; intros; apply listmaxZ_spec in H; omega).
+Defined.
